coq/src/Pearlite_Example.v
@@ -6,15 +6,103 @@ Import List.ListNotations.
 Open Scope Z_scope.
 Open Scope bool_scope.
 Open Scope hacspec_scope.
-Require Import Hacspec_Lib.
-Export Hacspec_Lib.
+Definition sum_first_n (n_0 : uint_size)  : uint_size :=
+  let sum_1 : uint_size :=
+    usize 0 in 
+  let sum_1 :=
+    foldi (usize 0) (n_0) (fun i_2 sum_1 =>
+      let sum_1 :=
+        (sum_1) + (i_2) in 
+      (sum_1))
+    sum_1 in 
+  sum_1.
 
-Definition ensure_something (x_0 : int8) (y_1 : int8)  `{x_0 = y_1} : bool :=
-  (x_0) =.? (y_1).
 
-Theorem ensures_ensure_something : forall result_2 (x_0 : int8) (y_1 : int8),
- forall {H_0 : x_0 = y_1},
- @ensure_something x_0 y_1 H_0 = result_2 ->
- ~ (result_2 = false).
- Proof. Admitted.
+Theorem ensures_sum_first_n : forall result_3 (n_0 : uint_size),
+ @sum_first_n n_0 = result_3 ->
+ result_3 = ((n_0) * ((n_0) - (usize 1))) / (usize 2).
+Proof.
+  intros. subst.
+
+  rewrite !nat_N_Z.
+  setoid_rewrite Z2Nat.id ; try easy.
+
+  Set Printing Coercions.
+
+  replace (unsigned (usize 1)) with 1 by reflexivity.
+  replace (unsigned (usize 2)) with 2 by reflexivity.
+
+  induction_uint_size_as_nat n_0.
+  - reflexivity.
+  - rewrite H1.
+    rewrite Z.sub_succ_l.
+
+    rewrite <- Zmult_succ_l_reverse.
+    rewrite <- Zmult_succ_r_reverse.
+
+    rewrite <- Zplus_assoc.
+    replace (Z.of_nat H + Z.succ (Z.of_nat H - 1))%Z with (Z.of_nat H * 2)%Z.
+    rewrite Z_div_plus.
+
+    unfold sum_first_n in H2 |- *.
+    unfold foldi in H2 |- *.
+    rewrite H1.
+    rewrite Z.sub_0_r in H2 |- *.
+
+    rewrite <- Zpos_P_of_succ_nat.
+
+    destruct H ; [ reflexivity | ].
+    rewrite Nat2Z.inj_succ in H2.
+    rewrite unsigned_repr_alt in H2.
+    rewrite <- Zpos_P_of_succ_nat in H2.
+    rewrite Zpos_P_of_succ_nat in H2.
+    rewrite SuccNat2Pos.id_succ in H2.
+
+    rewrite SuccNat2Pos.id_succ.
+    rewrite <- foldi__move_S_fuel.
+
+    assert (forall a b, Z_to_uint_size (a + b) = Z_to_uint_size (unsigned (Z_to_uint_size a) + unsigned (Z_to_uint_size b))).
+    intros.
+    cbn.
+    unfold Z_to_uint_size.
+    unfold repr.
+    apply mkint_eq.
+
+    rewrite !Z_mod_modulus_eq.
+    now rewrite Zplus_mod.
+
+    rewrite H3.
+    rewrite H2.
+    setoid_rewrite add_zero.
+    rewrite <- H3.
+    f_equal.
+
+    rewrite Nat2Z.inj_succ.
+
+    f_equal.
+    rewrite !nat_N_Z.
+    setoid_rewrite Z2Nat.id ; try easy.
+
+    rewrite unsigned_repr_alt.
+    reflexivity.
+    Lia.lia.
+
+    rewrite unsigned_repr_alt.
+    Lia.lia.
+    Lia.lia.
+
+    apply modulus_range_helper.
+    Lia.lia.
+
+    Lia.lia.
+
+    easy.
+
+    Lia.lia.
+  - destruct_uint_size_as_nat n_0.
+    easy. Lia.lia.
+  - destruct_uint_size_as_nat n_0.
+    easy. Lia.lia.
+Qed.
+
 
